Part 1 almost done

src/compil.fst
@@ -1,5 +1,14 @@
 module Compil
 
+val length: list 'a -> Tot nat
+let rec length l = match l with
+  | [] -> 0
+  | _ :: tl -> 1 + length tl
+
+let rec nth #a (l: list a) (n: nat{n < length l}) : a =
+    match l with 
+    | hd :: tl -> if n = 0 then hd else nth tl (n - 1)
+
 type deBruijn =
     | Var: nat -> deBruijn
     | Lambda: t:deBruijn -> deBruijn
@@ -59,3 +68,70 @@ let subst_clos (n: nat) (t: deBruijn{isClosed t}) (u: deBruijn):
     | Var i -> ()
     | App t' t'' -> subst_clos_aux n t' u; subst_clos_aux n t'' u
     | Lambda t' -> subst_clos_aux (n + 1) t' u
+
+let rec subst_mult_aux (t: deBruijn) (idx: nat) 
+    (u: list deBruijn): deBruijn =
+    let l = length u in
+    match t with 
+    | Var n -> 
+        if (n >= idx) && (n < l + idx) then nth u (n - idx)
+        else t
+    | Lambda t' -> 
+        Lambda (subst_mult_aux t' (idx + 1) u)
+    | App t' t'' -> 
+        App (subst_mult_aux t' idx u) (subst_mult_aux t'' idx u)
+
+let substMult (t: deBruijn) (idx: nat) (u: list deBruijn) =
+    subst_mult_aux t idx u
+
+let rec subst_mult_nil (t: deBruijn) (idx: nat):
+    Lemma (ensures ((substMult t idx []) = t)) =
+    match t with 
+    | Var n -> () 
+    | Lambda t' -> 
+        subst_mult_nil t' (idx + 1)
+    | App t' t'' -> 
+        subst_mult_nil t' idx; subst_mult_nil t'' idx
+
+let rec subst_mult_wd (t: deBruijn) (idx: nat) (u: deBruijn):
+    Lemma (ensures (
+        substitution t idx u = substMult t idx [u]
+    )) = 
+    match t with 
+    | Var i -> ()
+    | App t' t'' -> 
+        subst_mult_wd t' idx u; subst_mult_wd t'' idx u
+    | Lambda t' -> subst_mult_wd t' (idx + 1) u
+
+let rec subst_mult_close (i: nat) (t: deBruijn{genClosure t i})
+    (u: list deBruijn) :
+    Lemma (ensures ((substMult t i u) = t))
+    (decreases %[t; i]) = 
+    match t with
+    | Var n -> ()
+    | App t' t'' -> subst_mult_close i t' u; subst_mult_close i t'' u
+    | Lambda t' -> subst_mult_close (i + 1) t' u
+
+let rec list_closed (l: list deBruijn) (n: nat) =
+    match l with
+    | [] -> True
+    | t :: tl -> (genClosure t n) /\ (list_closed tl n)
+
+let rec subst_mult_pc (t: deBruijn) (n: nat) 
+    (ul: (list deBruijn){list_closed ul n}):
+    Lemma (ensures (
+        genClosure (substMult t n ul) n
+    )) = 
+    admit()
+
+let rec subst_mult_master (t: deBruijn) (n: nat)
+    (ul: (list deBruijn){list_closed ul n}) (u: deBruijn) :
+    Lemma (ensures (
+        (substMult t n (u :: ul)) = (substitution (substMult t (n + 1) ul) n u)
+    )) = 
+    match ul with 
+    | [] -> 
+        subst_mult_nil t n; 
+        subst_mult_pc t (n + 1) []; 
+        subst_mult_wd t n u; ()
+    | _ -> admit()
